backend/Linearizeproof.v
@@ -651,7 +651,8 @@ Proof.
   (* Lannot *)
   left; econstructor; split. simpl.
   apply plus_one. eapply exec_Lannot; eauto.
-  eapply external_call_symbols_preserved'; eauto.
+  eapply eval_annot_args_preserved with (ge1 := ge); eauto. exact symbols_preserved.
+  eapply external_call_symbols_preserved; eauto.
   exact symbols_preserved. exact public_preserved. exact varinfo_preserved.
   econstructor; eauto.
 
